{
  "@context": {
    "csvw": "http://www.w3.org/ns/csvw#",
    "anschema": "http://catalog.caida.org/ontology/anschema#",

    "description": {
      "@id": "anschema:description"
    },
    "entityUrl": {
      "@id": "anschema:entityUrl",
      "@type": "csvw:uriTemplate"
    },
    "name": {
      "@id": "anschema:name",
      "@language": null
    },
    "propertyUrl": {
      "@id": "aschema:propertyUrl",
      "@type": "csvw:uriTemplate"
    },
    "url": {
      "@id": "anschema:url",
      "@type": "xsd:anyURI"
    },

    "columnReference": {
      "@id": "anschema:columnReference",
      "@language": null,
      "@container": "@list"
    },
    "entityReference": {
      "@id": "anschema:columnReference",
      "@language": null,
      "@container": "@list"
    },

    "entities": {
      "@id": "anschema:entity",
      "@type": "@id",
      "@container": "@list"
    },
    "namespaceUrls": {
      "@id": "anschema:namespaceUrl",
      "@type": "@id",
      "@container": "@list"
    },
    "propertyMaps": {
      "@id": "anschema:propertyMap",
      "@type": "@id",
      "@container": "@list"
    }
  },
  "@graph": {
      "@context": {
      "id": "@id",
      "type": "@type",
      "dc:title": {
        "@container": "@language"
      },
      "dc:description": {
        "@container": "@language"
      },
      "dc:date": {
        "@type": "xsd:date"
      },
      "rdfs:comment": {
        "@container": "@language"
      },
      "rdfs:domain": {
        "@type": "@id"
      },
      "rdfs:label": {
        "@container": "@language"
      },
      "rdfs:range": {
        "@type": "@id"
      },
      "rdfs:seeAlso": {
        "@type": "@id"
      },
      "rdfs:subClassOf": {
        "@type": "@id"
      },
      "rdfs:subPropertyOf": {
        "@type": "@id"
      },
      "owl:equivalentClass": {
        "@type": "@vocab"
      },
      "owl:equivalentProperty": {
        "@type": "@vocab"
      },
      "owl:oneOf": {
        "@container": "@list",
        "@type": "@vocab"
      },
      "owl:imports": {
        "@type": "@id"
      },
      "owl:versionInfo": {
        "@type": "@id"
      },
      "owl:inverseOf": {
        "@type": "@vocab"
      },
      "owl:unionOf": {
        "@type": "@vocab",
        "@container": "@list"
      },
      "rdfs_classes": {
        "@reverse": "rdfs:isDefinedBy",
        "@type": "@id"
      },
      "rdfs_properties": {
        "@reverse": "rdfs:isDefinedBy",
        "@type": "@id"
      },
      "rdfs_datatypes": {
        "@reverse": "rdfs:isDefinedBy",
        "@type": "@id"
      },
      "rdfs_instances": {
        "@reverse": "rdfs:isDefinedBy",
        "@type": "@id"
      }
    },
    "@id": "http://catalog.caida.org/ontology/anschema#",
    "@type": "owl:Ontology",
    "dc:title": {
      "en": "CAIDA Annotated Schema Namespace Vocabulary Terms"
    },
    "dc:description": {
      "en": "CAIDA Annotated Schema is an extension to CSVW with the addition of Entities. Entities group together columns that share the same object and class."
    },
    "dc:date": "2023-05-01",
    "owl:imports": [
      "http://www.w3.org/ns/prov"
    ],
    "owl:versionInfo": "https://github.com/w3c/csvw/commit/fcc9db20ba4de10e41e964eee1b5d01defa4c664",
    "rdfs:seeAlso": [
      "http://www.w3.org/TR/tabular-metadata"
    ],
    "rdfs_classes": [
      {
        "@id": "anschema:Entity",
        "@type": "rdfs:Class",
        "rdfs:label": {
          "en": "Entity"
        },
        "rdfs:comment": {
          "en": "A Entity represents a group of columns that describe the same thing within a Table."
        }
      },
      {
        "@id": "anschema:Namespace",
        "@type": "rdfs:Class",
        "rdfs:label": {
          "en": "Namespace"
        },
        "rdfs:comment": {
          "en": "provides a guide to the set of class identifiers contained in the property"
        }
      },
      {
        "@id": "anschema:PropertyMap",
        "@type": "rdfs:Class",
        "rdfs:label": {
          "en": "PropertyMap"
        },
        "rdfs:comment": {
          "en": "A PropertyMap provides the mapping between the entity's class's property to a set of table columns."
        }
      }
    ],
    "rdfs_properties": [
      {
        "@id": "anschema:classUrl",
        "@type": "rdf:Property",
        "rdfs:label": {
          "en": "property URL"
        },
        "rdfs:comment": {
          "en": "An URI template class that provides the URI for a class defined for the Entity."
        },
        "rdfs:domain": "anschema:Entity",
        "rdfs:range": "csvw:uriTemplate"
      },
      {
        "@id": "anschema:columnReference",
        "@type": "rdf:Property",
        "rdfs:label": {
          "en": "column reference"
        },
        "rdfs:comment": {
          "en": "A column reference property that holds either a single reference to a column description object within the Entity or PropertyMap."
        },
        "rdfs:domain": {
          "owl:unionOf": [
            "anschema:Entity",
            "anschema:PropertyMap"
          ]
        },
        "rdfs:range": "xsd:string"
      },
      {
        "@id": "anschema:description",
        "@type": "rdf:Property",
        "rdfs:label": {
          "en": "name"
        },
        "rdfs:comment": {
          "en": "An account giving the characteristics of a Entity or Namespace."
        },
        "rdfs:domain": {
          "owl:unionOf": [
            "anschema:Entity",
            "anschema:Namespace"
          ]
        },
        "rdfs:range": "xsd:string"
      },
      {
        "@id": "anschema:entity",
        "@type": "rdf:Property",
        "rdfs:label": {
          "en": "entity"
        },
        "rdfs:comment": {
          "en": "An array property of  descriptions."
        },
        "rdfs:domain": "csvw:Schema",
        "rdfs:range": "anschema:Entity"
      },
      {
        "@id": "anschema:entityReference",
        "@type": "rdf:Property",
        "rdfs:label": {
          "en": "entity reference"
        },
        "rdfs:comment": {
          "en": "An Entity reference property that holds either a single reference to a Entity description object within the PropertyMap."
        },
        "rdfs:domain": "anschema:PropertyMap",
        "rdfs:range": "xsd:string"
      },
      {
        "@id": "anschema:label",
        "@type": "rdf:Property",
        "rdfs:label": {
          "en": "label"
        },
        "rdfs:comment": {
          "en": "This property is a shorter name annotation for the Entity or Namespace."
        },
        "rdfs:domain": {
          "owl:unionOf": [
            "anschema:Entity",
            "anschema:Namespace"
          ]
        },
        "rdfs:range": "xsd:string"
      },
      {
        "@id": "anschema:name",
        "@type": "rdf:Property",
        "rdfs:label": {
          "en": "name"
        },
        "rdfs:comment": {
          "en": "This property is the name annotation for the Entity or Namespace."
        },
        "rdfs:domain": {
          "owl:unionOf": [
            "anschema:Entity",
            "anschema:Namespace"
          ]
        },
        "rdfs:range": "xsd:string"
      },
      {
        "@id": "anschema:namespaceUrl",
        "@type": "rdf:Property",
        "rdfs:label": {
          "en": "namespace URL"
        },
        "rdfs:comment": {
          "en": "An URI template property that MAY be used to create one or more URI for a Namespaces for the property in the PropertyMap."
        },
        "rdfs:domain": "anschema:PropertyMap",
        "rdfs:range": "csvw:uriTemplate"
      },
      {
        "@id": "anschema:propertyMap",
        "@type": "rdf:Property",
        "rdfs:label": {
          "en": "entity"
        },
        "rdfs:comment": {
          "en": "An array property of PropertyMaps descriptions."
        },
        "rdfs:domain": "csvw:Entity",
        "rdfs:range": "anschema:PropertyMap"
      },
      {
        "@id": "anschema:propertyUrl",
        "@type": "rdf:Property",
        "rdfs:label": {
          "en": "property URL"
        },
        "rdfs:comment": {
          "en": "An URI template property that MAY be used to create a URI for a property in the PropertyMap."
        },
        "rdfs:domain": "anschema:PropertyMap",
        "rdfs:range": "csvw:uriTemplate"
      },
      {
        "@id": "anschema:url",
        "@type": "rdf:Property",
        "rdfs:label": {
          "en": "url"
        },
        "rdfs:comment": {
          "en": "A URL with more information on the Namespace."
        },
        "rdfs:domain": "anschema:url",
        "rdfs:range": "xsd:anyURI"
      }
    ]
 }
}
